src/PlutusIR/Semantics/Static/Normalisation/Progress.v
@@ -1,0 +1,122 @@
+
+(* Progress of the reduction relation used in the normaliser *)
+From PlutusCert Require Import PlutusIR Normalisation.Normalisation Kinding.Kinding Type_reduction
+Kinding.Checker.
+Require Import Coq.Lists.List.
+Import ListNotations.
+
+Axiom step_dec_SOP : forall l,
+  normal_Ty (Ty_SOP l).
+
+(* Need kinding because of e.g.
+  T = Ty_App (Ty_Fun Int Int) Int.
+  This is not normal (Ty_Fun is not neutral), and it also does not step (Ty_Fun not a Ty_lam)
+*)
+Definition step_dec (T : ty) : forall Δ K, has_kind Δ T K -> {T' & step T T'} + normal_Ty T.
+Proof.
+  induction T; intros.
+  - right.
+    repeat constructor.
+  - apply kind_checking_complete in H.
+    inversion H.
+    repeat destruct_match.
+    apply kind_checking_sound in Heqo.
+    apply kind_checking_sound in Heqo0.
+    edestruct IHT1; eauto.
+    + left. 
+      destruct s as [t1' Ht1].
+      exists (Ty_Fun t1' T2).
+      now constructor.
+    + edestruct IHT2; eauto.
+      * left.
+        destruct s as [t2' Ht2].
+        exists (Ty_Fun T1 t2').
+        now constructor.
+  
+  - apply kind_checking_complete in H.
+    inversion H.
+    repeat destruct_match.
+    apply kind_checking_sound in Heqo.
+    apply kind_checking_sound in Heqo0.
+    edestruct IHT1; eauto.
+    + left.
+      destruct s as [t1' Ht1].
+      exists (Ty_IFix t1' T2).
+      now constructor.
+    + edestruct IHT2; eauto.
+      left.
+      destruct s as [t2' Ht2].
+      exists (Ty_IFix T1 t2').
+      now constructor.
+  - apply kind_checking_complete in H. (* Note: Move to kind_checker world to fix not being able to `inversion` on `has_kind`*)
+    inversion H.
+    repeat destruct_match.
+    apply kind_checking_sound in Heqo.
+    destruct (IHT ((b, k) :: Δ) Kind_Base Heqo).
+    + left.
+      destruct s as [t1' Ht1].
+      exists (Ty_Forall b k t1').
+      now constructor.
+    + right.
+      apply NO_TyForall; assumption.
+  - right. apply NO_TyBuiltin. 
+  - apply kind_checking_complete in H. (* Note: Move to kind_checker world to fix not being able to `inversion` on `has_kind`*)
+    inversion H.
+    repeat destruct_match.
+    apply kind_checking_sound in Heqo.
+    destruct (IHT ((b, k) :: Δ) k0 Heqo).
+    + left.
+      destruct s as [t1' Ht1].
+      exists (Ty_Lam b k t1').
+      now constructor.
+    + right.
+      apply NO_TyLam; assumption.
+  - remember H as H_copy; clear HeqH_copy.
+    apply kind_checking_complete in H. (* Note: Move to kind_checker world to fix not being able to `inversion` on `has_kind`*)
+    inversion H.
+    repeat destruct_match.
+    apply kind_checking_sound in Heqo.
+    destruct (IHT1 Δ (Kind_Arrow k0_1 k0_2) Heqo).
+    + left.
+      destruct s as [t1' Ht1].
+      exists (Ty_App t1' T2).
+      now constructor.
+    + apply kind_checking_complete in H_copy. (* Note: Move to kind_checker world to fix not being able to `inversion` on `has_kind`*)
+      inversion H.
+      repeat destruct_match.
+      apply kind_checking_sound in Heqo2.
+      destruct (IHT2 Δ k2 Heqo2).
+      * left.
+        destruct s as [t2' Ht2].
+        exists (Ty_App T1 t2').
+        now constructor.
+      * 
+        {
+        induction T1.
+        - right. constructor. constructor.
+          + inversion n. assumption.
+          + assumption.
+        - (* This does not step *)
+          (* but this is also never a normal ty since Ty_Fun is never neutral*)
+          exfalso.
+          (* it must be ill-kinded *)
+          inversion Heqo.
+        - exfalso. 
+          inversion Heqo.
+        - exfalso.
+          inversion Heqo.
+        - exfalso. 
+          inversion Heqo.
+        - left. 
+          exists (substituteTCA b T2 T1).
+          constructor.
+          + inversion n. assumption. inversion H0.
+          + assumption.
+        - right. constructor. constructor.
+          + inversion n. assumption.
+          + assumption.
+        - apply Checker.prop_to_type in Heqo. inversion Heqo.
+        }
+  - right. apply step_dec_SOP. (* TODO: Different induction prniciple! *)
+Defined.
+
