src/PlutusIR/Semantics/Static/Normalisation/Strong_Normalisation/SN_STLC/SN_STLC_GU/GU_NC_Uhm.v
@@ -1,0 +1,372 @@
+From mathcomp Require Import ssreflect ssrbool eqtype ssrnat.
+From Coq Require Import ssrfun.
+Require Import Coq.Strings.String.
+Require Import Coq.Lists.List.
+From PlutusCert Require Import Util.List.
+Import ListNotations.
+Local Open Scope string_scope.
+Local Open Scope list_scope.
+Require Import Lia.
+Require Import Coq.Program.Basics.
+Require Import Coq.Arith.Arith.
+
+From PlutusCert Require Import STLC step_naive util alpha.alpha variables alpha_freshness alpha_ctx_sub.
+
+
+
+Create HintDb α_eq_db.
+Hint Constructors Alpha : α_eq_db.
+Hint Resolve alpha_refl : α_eq_db.
+Hint Resolve alpha_sym : α_eq_db.
+Hint Resolve alpha_trans : α_eq_db.
+Hint Constructors AlphaCtxRefl : α_eq_db.
+Hint Constructors AlphaVar : α_eq_db.
+Hint Constructors αCtxSub : α_eq_db.
+Hint Constructors AlphaCtxSym : α_eq_db.
+Hint Constructors αCtxTrans : α_eq_db.
+Hint Resolve alpha_extend_ids : α_eq_db.
+Hint Constructors IdCtx : α_eq_db.
+Hint Resolve sym_alpha_ctx_is_sym : α_eq_db.
+Hint Resolve sym_alpha_ctx_is_sym : α_eq_db.
+Hint Resolve sym_alpha_ctx_left_is_sym  : α_eq_db.
+
+
+(* 
+Lemma remove_ids_subset sigma :
+  incl (remove_ids sigma) sigma.
+Proof.
+  unfold incl.
+  intros.
+  induction sigma.
+  - inversion H.
+  - 
+    (* need lemma to rewrite a in remove_ids a0 :: sigma to a in a0 :: remove_ids sigma*)
+    admit.
+Admitted.
+
+
+
+Lemma remove_ids_helper2 sigma s s' :
+  In (s, tmvar s') sigma -> s <> s' -> In (s, tmvar s') (remove_ids sigma).
+Proof.
+  intros.
+  induction sigma; auto.
+  destruct a as [a1 a2].
+  simpl.
+  induction a2.
+  - destr_eqb_eq a1 s0. eapply IHsigma.
+    inversion H. inversion H1; subst. contradiction.
+    auto.
+    inversion H. inversion H2; subst. apply in_eq. apply in_cons.
+    eapply IHsigma; auto.
+  - apply in_cons.
+    eapply IHsigma; eauto.
+    inversion H; intuition.
+    inversion H1.
+  - apply in_cons.
+    eapply IHsigma; eauto.
+    inversion H; intuition.
+    inversion H1.
+  - apply in_cons.
+    eapply IHsigma; eauto.
+    inversion H; intuition.
+    inversion H1.
+Qed. *)
+
+
+(* So sub is also rewritten when rewriting subs *)
+Hint Extern 1 => simpl sub : subs_db.
+
+Inductive GU : term -> Set :=
+| GU_var x : GU (tmvar x)
+(* in app, if s and t do not share GU_vars: *)
+| GU_app {B} s t : 
+    GU s -> 
+    GU t -> 
+    forall (H_btv_btv_empty : forall x, In x (btv t) -> ~ In x (tv s)),
+    forall (H_btv_ftv_empty : forall x, In x (btv s) -> ~ In x (tv t)),
+    GU (@tmapp B s t)
+| GU_lam {B} x A s : 
+    GU s -> 
+    ~ In x (btv s) ->
+    GU (@tmlam B x A s)
+| GU_builtin d :
+    GU (tmbuiltin d).
+
+(* Not sure how to call this yet.
+if we have NC t sigma
+We want to have unique binders elementwise in sigma.
+No binder in t can occur as free or bound variable in sigma,
+  thus substituting sigma in t will not cause unwanted capture.
+*)
+Inductive NC : term -> list (string * term) -> Set :=
+| nc_nil s :
+    NC s []
+| nc_cons s x t sigma :
+    NC s sigma ->
+    (forall y, In y (btv s) -> ((y <> x) * (~ In y (ftv t)))) -> (* no capturing *)
+    NC s ((x, t) :: sigma).
+
+Lemma nc_smaller {s sigma x t} : NC s ((x, t)::sigma) -> NC s sigma.
+Proof.
+  intros.
+  inversion H; subst.
+  auto.
+Qed.
+
+(* why doesnt sigma grow???
+  NC: forall btv in s, not in sigma
+  we remove a binder, thenw e should still have that all remaining btvs are not in the original sigma.
+*)
+Lemma nc_lam {B x s A sigma} : 
+  NC (@tmlam B x A s) sigma -> NC s sigma.
+Proof.
+  induction sigma; [constructor|]; intros Hnc.
+  inversion Hnc; subst.
+  constructor.
+  + eapply IHsigma. auto.
+  + intros y H_btvs.
+    eapply btv_c_lam in H_btvs; eauto.
+Qed.
+
+Lemma nc_app_l {B s t sigma} :
+  NC (@tmapp B s t) sigma -> NC s sigma.
+Proof.
+  induction sigma; [constructor|]; intros Hnc.
+  inversion Hnc; subst.
+  constructor.
+  + eapply IHsigma. auto.
+  + intros y H_btvs.
+    eapply btv_c_appl in H_btvs; eauto.
+Qed.
+
+Lemma nc_app_r {B s t sigma} :
+  NC (@tmapp B s t) sigma -> NC t sigma.
+Proof.
+  induction sigma; [constructor|]; intros Hnc.
+  inversion Hnc; subst.
+  constructor.
+  + eapply IHsigma. auto.
+  + intros y H_btvs.
+    eapply btv_c_appr in H_btvs; eauto.
+Qed.
+
+(* No free vars are changed *)
+Lemma alpha_preserves_nc_ctx s x t t':
+   Alpha [] t t' -> NC s ((x, t)::nil) -> NC s ((x, t')::nil).
+Proof.
+  intros Ha_t Hnc_t.
+  inversion Hnc_t; subst.
+  constructor. auto.
+  intros y Hbtv.
+  specialize (H4 y Hbtv).
+  destruct H4 as [Hynotx Hftv_t].
+  split; auto.
+  eapply alpha_preserves_no_ftv; eauto.
+  constructor.
+Qed.
+
+Lemma gu_app_l {B s t} :
+  GU (@tmapp B s t) -> GU s.
+Proof.
+  inversion 1; auto.
+Qed.
+
+Lemma gu_app_r {B s t} :
+  GU (@tmapp B s t) -> GU t.
+Proof.
+  inversion 1; auto.
+Qed.
+
+Lemma gu_lam {B x A s} :
+  GU (@tmlam B x A s) -> GU s.
+Proof.
+  inversion 1; auto.
+Qed.
+
+Lemma gu_app_st__gu_app_ts {B} s1 s2 :
+  GU (@tmapp B s1 s2) -> GU (@tmapp B s2 s1).
+Proof.
+  intros.
+  inversion H; subst.
+  constructor; auto.
+Qed.
+
+Lemma gu_applam_to_nc {BA} {BL} s t x A :
+  GU (@tmapp BA (@tmlam BL x A s) t) -> NC s [(x, t)].
+Proof.
+  intros Hgu.
+  inversion Hgu as [ | ? ? ? Hgu_lam Hgu_t Hgu_P1 Hgu_P2 | | ]; subst.
+  repeat constructor.
+  - intros Hcontra; subst.
+    inversion Hgu_lam; subst.
+    contradiction.
+  - intros Hcontra; apply extend_ftv_to_tv in Hcontra; revert Hcontra.
+    apply Hgu_P2.
+    apply btv_c_lam; auto.
+Qed.
+
+(* The fundamental NC property*)
+Lemma nc_ftv_env s sigma :
+  NC s sigma -> forall x, In x (btv s) -> ~ In x (ftv_keys_env sigma).
+Proof.
+  intros Hnc x Hin_btvs.
+  induction Hnc.
+  - simpl. auto.
+  - simpl.
+    specialize (p x Hin_btvs) as [Hnotx Hnott].
+    apply de_morgan2.
+    split; auto.
+    apply not_in_app.
+    split; auto.
+Qed.
+
+
+Lemma gu_ftv_then_no_btv s x :
+  GU s -> In x (ftv s) -> ~ In x (btv s).
+Proof.
+  intros Hgu Hins.
+  induction Hgu.
+  - simpl in Hins. auto.
+  - simpl in Hins.
+    apply in_app_iff in Hins as [Hins | Hins].
+    + simpl.
+      apply not_in_app.
+      split.
+      * auto.
+      * intros Hcontra.
+        apply H_btv_btv_empty in Hcontra.
+        apply extend_ftv_to_tv in Hins.
+        contradiction.
+    + simpl.
+      apply not_in_app.
+      split.
+      * intros Hcontra.
+        apply H_btv_ftv_empty in Hcontra.
+        apply extend_ftv_to_tv in Hins.
+        contradiction.
+      * auto.
+  - simpl.
+    apply de_morgan2.
+    split.
+    + intros Hcontra.
+      subst.
+      apply ftv_lam_no_binder in Hins. 
+      auto.
+    + apply IHHgu.
+      apply ftv_lam_helper in Hins.
+      auto.
+  - inversion Hins.
+Qed.
+
+
+Lemma step_naive_preserves_nc_ctx s t1 t2 x :
+  step_naive t1 t2 -> NC s ((x, t1)::nil) -> NC s ((x, t2)::nil).
+Proof.
+  intros Hstep Hnc.
+  inversion Hnc; subst.
+  constructor.
+  - constructor.
+  - intros y Hbtv.
+    specialize (H4 y Hbtv).
+    destruct H4 as [Hynotx Hftv_t].
+    split; auto.
+    eapply step_naive_preserves_no_ftv. eauto. auto.
+Qed.
+
+
+(* Two properties: stopping clash between sigma and s:
+  forall x binder in sigma, we rename it in t, hence we need to add that name to R.
+  Hence it cannot be free in s, otherwise we no longer have R ⊢ s ~ s.
+  We use tv instead of ftv because that decomposes over lam, while we still allow identity substitutions
+
+  Second property: when x is a btv in sigma, then it is not an ftv in sigma.
+    e.g. if x is a binder, then we need to rename that in t.
+      so then we dont want that same x to also occur free (or as key) in sigma, because then we no longer have
+      R ⊢ sigma ~ sigma
+
+    Since identity substitutions have no binders, this still allows for identity substitutions.
+    In the lam case we extend sigma with (X, t').
+      - X: X was a binder in s, hence a tv in s. So it was not in btv_env_sigma by first condition
+      - t': we have control over binders in t', so that is no problem. But for all other binders already in sigma,
+            we also need that they don't clash with ftvs in t'. But this is exactly what we are renaming in t':
+              those ftv in t' that are binders in sigma! 
+
+    This argument is tooooo subtle, need to formalise.
+    What about ftv in t that are also ftv in s? they are not renamed and thus in t'.
+     Can they be btv in sigma? No by the first argument
+
+*)
+
+(* Property that allows to add binder names (a, b, c,...) to alpha context R, and keeping the property that
+    R ⊢ s ~ s, and R ⊢ sigma ~ sigma
+   - binders in sigma are not free in s
+   - binders in sigma are not free in sigma
+   - binders in s are not free in sigma, exactly NC s sigma: so moved out of this
+*)
+Definition Uhm sigma s := ((forall x, In x (btv_env sigma) -> ~ In x (tv s)) 
+  * (forall x, In x (btv_env sigma) -> ~ In x (ftv_keys_env sigma)))%type.
+
+Lemma uhm_smaller {sigma s x t} : Uhm ((x, t)::sigma) s -> Uhm sigma s.
+Proof.
+  intros.
+  unfold Uhm.
+  split; unfold Uhm in H; destruct H as [ uhm1 uhm2]; intros.
+  - eapply uhm1.
+    simpl. apply in_app_iff. right. assumption.
+  - assert (~ In x0 (ftv_keys_env ((x, t)::sigma))).
+    {
+      eapply uhm2.
+      simpl. apply in_app_iff. right. assumption.
+    }
+    simpl in H0.
+    intuition.
+Qed.
+
+
+Lemma Uhm_appl {B s t sigma} :
+  Uhm sigma (@tmapp B s t) -> Uhm sigma s.
+Proof.
+  intros.
+  unfold Uhm in H.
+  destruct H as [ uhm1 uhm2].
+  unfold Uhm.
+  split; intros.
+  - specialize (uhm1 x H).
+    apply not_tv_dc_appl in uhm1. auto.
+  - specialize (uhm2 x H). auto.
+Qed.
+
+Lemma Uhm_appr {B s t sigma} :
+  Uhm sigma (@tmapp B s t) -> Uhm sigma t.
+Proof.
+  intros Huhm.
+  unfold Uhm in Huhm.
+  destruct Huhm as [ uhm1 uhm2].
+  unfold Uhm.
+  split; intros.
+  - specialize (uhm1 x H).
+    apply not_tv_dc_appr in uhm1. auto.
+  - specialize (uhm2 x H). auto.
+Qed.
+
+(* x not in btv s, hence we can add it freely as ftv to sigma*)
+Lemma Uhm_lam_id {B x A s sigma} :
+  GU (@tmlam B x A s) ->
+  (* cannot combine uhm3 and uhm1: free vars in t can still be free vars in s*)
+  Uhm sigma (@tmlam B x A s) -> Uhm ((x, tmvar x)::sigma) s.
+Proof.
+  intros Hgu Huhm.
+  unfold Uhm in Huhm.
+  destruct Huhm as [ uhm1 uhm2].
+  unfold Uhm.
+  split; intros.
+  - eapply not_tv_dc_lam.
+    eapply uhm1. auto.
+  - simpl in H.
+    simpl.
+    apply de_morgan2.
+    split; [|apply de_morgan2; split].
+    all: try solve [intros Hcontra; subst; apply uhm1 in H; simpl in H; intuition].
+    now apply uhm2.
+Qed.
