src/PlutusIR/Semantics/Static/Normalisation/Strong_Normalisation/SN_STLC/SN_STLC_GU/IdSubst.v
@@ -1,0 +1,111 @@
+Require Import Coq.Lists.List.
+Import ListNotations.
+Require Import Coq.Strings.String.
+Require Import PlutusCert.PlutusIR.Semantics.Static.Normalisation.Strong_Normalisation.SN_STLC.SN_STLC_GU.psubs.
+
+From PlutusCert Require Import GU_NC_Uhm STLC util variables.
+
+
+Inductive IdSubst : list (string * term) -> Set :=
+  | id_subst_nil : IdSubst nil
+  | id_subst_cons : forall x sigma , IdSubst sigma -> IdSubst ((x, tmvar x)::sigma).
+
+
+Lemma id_subst__id s σ :
+  (* NC s σ ->  *)
+  IdSubst σ -> 
+  psubs σ s = s. (* even when this capturs, it doesnt matter, since it captures something and then substiutes it for the same name*)
+Proof.
+  intros.
+  induction s.
+  - induction σ.
+    + reflexivity.
+    + simpl. destruct a as [x1 x2].
+      inversion H; subst.
+      specialize (IHσ H1).
+      simpl in IHσ.
+      destr_eqb_eq x1 s; auto.
+  - simpl.
+    f_equal.
+    apply IHs.
+  - simpl.
+    f_equal; eauto.
+  - simpl; auto.
+Qed.
+
+
+(* Identity substitutions: Given a typing context E, give a list of term substitutions matching this E*)
+Fixpoint id_subst (E : list (string * PlutusIR.kind)) : list (string * term) :=
+  match E with
+  | nil => nil
+  | cons (x, A) E' => cons (x, tmvar x) (id_subst E')
+  end.
+
+
+Lemma id_subst_is_IdSubst E :
+  IdSubst (id_subst E).
+Proof.
+  induction E.
+  - constructor.
+  - simpl. destruct a. constructor. assumption.
+Qed.
+
+Lemma remove_ids_IdSubst_is_nil sigma :
+  IdSubst sigma -> remove_ids sigma = nil.
+Proof.
+  intros.
+  induction sigma.
+  - reflexivity.
+  - simpl.
+    destruct a as [x1 x2].
+    inversion H; subst.
+    rewrite IHsigma; auto.
+    rewrite String.eqb_refl. auto.
+Qed.
+
+Lemma IdSubst_no_binders sigma :
+  IdSubst sigma -> btv_env sigma = nil.
+Proof.
+  intros.
+  induction sigma.
+  - reflexivity.
+  - simpl.
+    destruct a as [x1 x2].
+    inversion H; subst.
+    rewrite IHsigma; auto.
+Qed.
+
+Lemma id_subst__ParSeq :
+  forall (σ : list (string * term)), IdSubst σ -> ParSeq σ.
+Proof.
+  intros.
+  induction σ.
+  - constructor.
+  - simpl. destruct a as [x1 x2]. constructor. 
+    + apply IHσ. inversion H. assumption.
+    + inversion H; subst.
+      rewrite (remove_ids_IdSubst_is_nil _ H1). auto.
+    + inversion H; subst.
+      rewrite IdSubst_no_binders; eauto.
+Qed.
+
+Lemma no_btv_in_id_subst E :
+  forall x, In x (btv_env (id_subst E)) -> False.
+Proof.
+  intros.
+  induction E.
+  - simpl in H. contradiction.
+  - simpl in H. destruct a as [x1 x2].
+    simpl in H.
+    eapply IHE. auto.
+Qed.
+
+Lemma id_subst__nc_uhm E s :
+  NC s (id_subst E) -> Uhm (id_subst E) s.
+Proof.
+  intros.
+  unfold Uhm.
+  split.
+  - intros. apply no_btv_in_id_subst in H0. contradiction.
+  - intros. apply no_btv_in_id_subst in H0. contradiction.
+Qed.
