src/PlutusIR/Semantics/Static/Normalisation/Strong_Normalisation/SN_STLC/SN_STLC_GU/step_naive.v
@@ -1,0 +1,128 @@
+Require Import Coq.Strings.String.
+Require Import Coq.Lists.List.
+Import ListNotations.
+From PlutusCert Require Import STLC util variables Util
+  Util.List psubs.
+
+Local Open Scope string_scope.
+
+Fixpoint sub (X : string) (U T : term) : term :=
+  match T with
+  | tmvar Y =>
+    if X =? Y then U else tmvar Y
+  | @tmlam B Y K1 T' =>
+    @tmlam B Y K1 (sub X U T') (* X can never be equal to Y due to GU: We only ever do substitutions such that NC T [(X, U)]*)
+  | @tmapp B T1 T2 =>
+    @tmapp B (sub X U T1) (sub X U T2)
+  | tmbuiltin d => tmbuiltin d
+  end.
+
+
+Lemma single_subs_is_psub X T s :
+  psubs [(X, T)] s = sub X T s.
+Proof.
+  induction s.
+  - simpl. destr_eqb_eq X s. reflexivity.
+    reflexivity.
+  - simpl. f_equal. apply IHs.
+  - simpl. f_equal. apply IHs1. apply IHs2.
+  - simpl. reflexivity.
+Qed.
+
+Lemma sub_helper {x t s} :
+  ~ In x (ftv t) -> ~ In x (ftv (sub x t s)).
+Proof.
+  intros Hcontra.
+  induction s.
+  - destr_eqb_eq x s.
+    + simpl. destr_eqb_eq s s. auto. contradiction.
+    + simpl. destr_eqb_eq x s. auto.
+      intros Hcontra2.
+      apply ftv_var in Hcontra2. contradiction.
+  - simpl. (* remove_string_dec s (ftv (sub x t s0)) is a subset of ftv (sub x t s0)*)
+    intros Hcontra2.
+    apply in_remove in Hcontra2.
+    destruct Hcontra2 as [Hcontra2 _].
+    contradiction.
+  - simpl. apply not_in_app. split.
+    + apply IHs1.
+    + apply IHs2.
+  - simpl. auto.
+Qed.
+
+(* need also handle btv, since substitution is nto capture avoiding*)
+Lemma sub_vac x t s :
+ ~ In x (ftv s) ->
+ ~ In x (btv s) ->
+ sub x t s = s.
+Proof.
+  intros.
+  induction s; simpl; auto.
+  - destr_eqb_eq x s; auto.
+    unfold ftv in H. contradiction H. apply in_eq.
+  - f_equal.
+    assert (~ In x (ftv s0)).
+    {
+      simpl in H0.
+      apply ftv_lam_negative in H; auto.
+    }
+    specialize (IHs H1 (not_btv_dc_lam H0)). auto.
+  - f_equal.
+    + eapply IHs1; eauto.
+      eapply not_ftv_app_not_left; eauto. eapply not_btv_dc_appl. eauto.
+    + eapply IHs2; eauto.
+      eapply not_ftv_app_not_right; eauto. eapply not_btv_dc_appr. eauto.
+Qed.
+(* looks like sub_vacuous maybe?*)
+
+Inductive step_naive : term -> term -> Set :=
+| step_beta (x : string) (A : PlutusIR.kind) (s t : term) :
+    step_naive (@tmapp App (@tmlam Lam x A s) t) ( sub x t s)
+| step_appL B s1 s2 t :
+    step_naive s1 s2 -> step_naive (@tmapp B s1 t) (@tmapp B s2 t)
+| step_appR B s t1 t2 :
+    step_naive t1 t2 -> step_naive (@tmapp B s t1) (@tmapp B s t2)
+| step_abs B x A s1 s2 :
+    step_naive s1 s2 -> step_naive (@tmlam B x A s1) (@tmlam B x A s2).
+
+
+Lemma step_naive_preserves_no_ftv x t1 t2 :
+  step_naive t1 t2 -> ~ In x (ftv t1) -> ~ In x (ftv t2).
+Proof.
+  intros Hstep Hftv_t1.
+  induction Hstep.
+  - destr_eqb_eq x x0.
+    + apply sub_helper. apply not_ftv_app_not_right in Hftv_t1. auto.
+    + rewrite <- single_subs_is_psub.
+      apply psubs_does_not_create_ftv.
+      * apply not_ftv_app_not_left in Hftv_t1. auto. eapply ftv_lam_negative; eauto.
+      * unfold ftv_keys_env. simpl. apply not_in_cons. split.
+        -- auto.
+        -- apply not_ftv_app_not_right in Hftv_t1. rewrite app_nil_r. auto.
+  - specialize (IHHstep (not_ftv_app_not_left Hftv_t1)).
+    intros Hcontra.
+    simpl in Hcontra.
+    apply in_app_or in Hcontra.
+    destruct Hcontra.
+    + apply IHHstep in H.
+      contradiction.
+    + apply not_ftv_app_not_right in Hftv_t1.
+      contradiction.
+  - specialize (IHHstep (not_ftv_app_not_right Hftv_t1)).
+    intros Hcontra.
+    simpl in Hcontra.
+    apply in_app_or in Hcontra.
+    destruct Hcontra.
+    + apply not_ftv_app_not_left in Hftv_t1.
+      contradiction.
+    + apply IHHstep in H.
+      contradiction.
+  - destr_eqb_eq x0 x.
+    + apply ftv_lam_no_binder.
+    + intros Hcontra.
+      apply ftv_lam_helper in Hcontra.
+      apply ftv_lam_negative in Hftv_t1.
+      specialize (IHHstep Hftv_t1).
+      contradiction. auto.   
+Qed.
+
