src/PlutusIR/Semantics/Static/Normalisation/Strong_Normalisation/SN_STLC/alpha/alpha_rename.v
@@ -1,7 +1,7 @@
 Require Import Coq.Strings.String.
 Require Import Coq.Lists.List.
 Import ListNotations.
-From PlutusCert Require Import STLC_named alpha.alpha Util.List freshness util.
+From PlutusCert Require Import STLC alpha.alpha Util.List variables util.
 Local Open Scope string_scope.
 Local Open Scope list_scope.
 
@@ -160,68 +160,3 @@ Proof.
     apply alphaRename.
     now apply fresh2_over_tv_term in H.
 Qed.
-
-(* alpha contexts and renaming contexts work the same with shadowing, so this holds
-  e.g. if R = (x, y)::(x, z), then mren will rename x to y.
-  Also Alpha (x, y)::(x, z) x y holds
-  Since the rhs of R can never occur in s, we know that also then z cannot occur in (mren R s)
-*)
-Lemma alpha_mren (R : list (string * string)) s :
-  (* x' can be equal to x., but then x=x' not in s, so the renaming doesnt do anything. *)
-  (forall x, In x (map snd R) -> ~ In x (ftv s)) -> Alpha R s (mren R s).
-Proof.
-Admitted.
-
-
-(* what we want is:
-Suppose   s = (x, y)
-Suppose R = (x, y), then that is problematic of course (the y is already present)
-But, if R is extended with (y, yfr), then this is no longer problematic.
-In other words we need:
-forall x, In x (map snd R) AND  In fst s  ->  Either: it is later somewhere in (fst R), i.e.: it gets fixed away
-
-Thought experiment:
-what if it gets fixed away to some other free var in s? Then it has to do this formula again, and needs to get fixed away again
-Because it is folding over the structure, at some point it needs to be translated to something not in the ftvs
-
-ok. What about
-s = (x, y)
-R = (x, y), (y, x)
-should not be problematic. But why/how to encode this?
-
-
-Hmm. I guess we could make sure that forall ftvs in s (in the original problem), we have a renaming in R (can be identity)
-Then we can rename every ftv at the end of R to something fresh => then we can never have "capture"
-*)
-Lemma alpha_mren_hmm (R : list (string * string)) s :
-  (* x' can be equal to x., but then x=x' not in s, so the renaming doesnt do anything. *)
-  (forall x, In x (map snd R) -> ~ In x (ftv s)) -> Alpha R s (mren R s).
-Proof.
-Admitted.
-
-(* Renamings can be faulty if we rename to something (say y) and y already occured in the term
-  this inductive makes sure that when this occurs the "original" y also gets renamed to something unproblematic
-*)
-Inductive Nice : (list (string * string)) -> term -> Prop :=
-  | NiceNil t : Nice nil t
-
-  (* If we rename something to y, and that already occured in t, then we need to rename that away thereafter*)
-  | NiceOne x y t R :  ~ In y (btv t) ->   In y (ftv t) -> In y (map fst R) -> Nice R t -> Nice ((x, y)::R) t
-  | NiceTwo x y t R : ~ In y (btv t) -> ~ In y (ftv t) ->                     Nice R t -> Nice ((x, y)::R) t. (* Not a problematic renaming*)
-(* for non-problematic renamings it can also not be in a bound type variable:
-  look at R = (x, y) and t = (tmlam y. x).
-*)
-
-(*
-  If R is nice, then the renaming is capture-avoiding.
-
-  Forall R, we can create R' which is Nice by extending R with renaming all ftvs to fresh vars, that is the key here
-  Also, if we extend R with identity substitutions, we can thereafter still do the extending by freshes.
-  If already (x, y), (y, x) in R. And we extend with (x, xfr), (y, yfr), then this does nothing (shadowed)
-  but what it does do is have an easy way of always knowing the renaming will be ok: we are playing on the safe side
-*)
-
-(* oooof.. Nice allows R = (x, y) and s = tmlam y. x y. Problem is that the rhs is a btv there.
-  I think an "easy" fix is to assume nothing in rhs R appears in btv of s.
-  I have nwo put this into nice
- *)
